Foundation/Modal/Neighborhood/AxiomC.lean
@@ -12,6 +12,22 @@ class Frame.IsRegular (F : Frame) : Prop where
 
 lemma Frame.regular [Frame.IsRegular F] {X Y : Set F} : (F.box X) ∩ (F.box Y) ⊆ F.box (X ∩ Y) := by apply IsRegular.regular
 
+open Classical in
+lemma Frame.regular_finset_iUnion [F.IsRegular] (s : Finset (Set F)) (hs : s.Nonempty) : (⋂ i ∈ s, F.box i) ⊆ F.box (⋂ i ∈ s, i) := by
+  induction s using Finset.induction_on with
+  | empty => simp_all;
+  | insert i s hi ih =>
+    wlog hs : s.Nonempty;
+    . simp_all;
+    replace ih := ih hs;
+    apply Set.Subset.trans ?_ (show i ∩ ⋂ j ∈ s, j = ⋂ j ∈ insert i s, j by simp ▸ F.regular (X := i) (Y := ⋂ j ∈ s, j));
+    suffices (F.box i) ∩ (⋂ j ∈ s, F.box j) ⊆ F.box (⋂ j ∈ s, j) by simpa;
+    grind;
+
+open Classical in
+lemma Frame.regular_finite_iUnion [F.IsRegular] {ι} [h : Fintype ι] [Nonempty ι] {X : ι → Set F} : (⋂ i : ι, F.box (X i)) ⊆ F.box (⋂ i : ι, X i) := by
+  simpa using Frame.regular_finset_iUnion (Finset.univ.image X) (by simp);
+
 instance : Frame.simple_blackhole.IsRegular := ⟨by
   intro X Y e;
   simp_all;
@@ -45,15 +61,14 @@ instance : (minimalCanonicalFrame 𝓢).IsRegular := by
   rintro X Y Γ ⟨hX, hY⟩;
   obtain ⟨φ, rfl, hφ⟩ := minimalCanonicalFrame.exists_box X Γ hX;
   obtain ⟨ψ, rfl, hψ⟩ := minimalCanonicalFrame.exists_box Y Γ hY;
-  rw [(show proofset 𝓢 φ ∩ proofset 𝓢 ψ = proofset 𝓢 (φ ⋏ ψ) by simp)];
+  suffices Γ ∈ proofset 𝓢 (□(φ ⋏ ψ)) by
+    rwa [(show proofset 𝓢 φ ∩ proofset 𝓢 ψ = proofset 𝓢 (φ ⋏ ψ) by grind), minimalCanonicalFrame.box_proofset];
   have : proofset 𝓢 (□φ ⋏ □ψ) ⊆ proofset 𝓢 (□(φ ⋏ ψ)) := proofset.imp_subset |>.mp (by simp);
-  have : Γ ∈ proofset 𝓢 (□(φ ⋏ ψ)) := this $ by
+  exact this $ by
     simp only [proofset.eq_and, Set.mem_inter_iff];
     constructor;
     . apply hφ ▸ hX;
     . apply hψ ▸ hY;
-  convert this;
-  convert Frame.IsCanonical.box_proofset (F := minimalCanonicalFrame 𝓢) (𝓢 := 𝓢) (φ ⋏ ψ);
 
 end
 
