Foundation/Modal/Neighborhood/Filtration.lean
@@ -1,0 +1,622 @@
+/-
+  Filtration of neighborhood semantics.
+
+  References:
+  - K. Kopnev, "The Finite Model Property of Some Non-normal Modal Logics with the Transitivity Axiom", https://arxiv.org/abs/2305.08605
+-/
+
+import Mathlib.Data.Set.Finite.Powerset
+import Foundation.Modal.Neighborhood.AxiomGeach
+import Foundation.Modal.Neighborhood.Supplementation
+import Foundation.Modal.Neighborhood.IntersectionClosure
+
+namespace LO.Modal
+
+namespace Neighborhood
+
+open FormulaSet.IsSubformulaClosed
+open Formula (atom)
+open Formula.Neighborhood
+
+attribute [grind]
+  FormulaSet.IsSubformulaClosed.of_mem_imp₁
+  FormulaSet.IsSubformulaClosed.of_mem_imp₂
+  FormulaSet.IsSubformulaClosed.of_mem_box
+
+variable {M : Model} {T : FormulaSet ℕ} [T.IsSubformulaClosed] {x y : M.World} {φ ψ : Formula ℕ}
+
+def filterEquiv (M : Model) (T : FormulaSet ℕ) [T.IsSubformulaClosed] (x y : M.World) := ∀ φ, (_ : φ ∈ T) → x ⊧ φ ↔ y ⊧ φ
+
+lemma filterEquiv.equivalence (M : Model) (T : FormulaSet ℕ) [T.IsSubformulaClosed] : Equivalence (filterEquiv M T) where
+  refl := by intro x φ _; rfl;
+  symm := by intro x y h φ hp; exact h _ hp |>.symm;
+  trans := by
+    intro x y z exy eyz;
+    intro φ hp;
+    exact Iff.trans (exy φ hp) (eyz φ hp)
+
+def FilterEqvSetoid (M : Model) (T : FormulaSet ℕ) [T.IsSubformulaClosed] : Setoid (M.World) := ⟨filterEquiv M T, filterEquiv.equivalence M T⟩
+
+abbrev FilterEqvQuotient (M : Model) (T : FormulaSet ℕ) [T.IsSubformulaClosed] := Quotient (FilterEqvSetoid M T)
+
+namespace FilterEqvQuotient
+
+@[grind]
+lemma iff_eq : (⟦x⟧ : FilterEqvQuotient M T) = ⟦y⟧ ↔ (∀ φ ∈ T, x ⊧ φ ↔ y ⊧ φ) := by
+  simp [FilterEqvSetoid, filterEquiv];
+
+lemma finite (T_finite : T.Finite) : Finite (FilterEqvQuotient M T) := by
+  have : Finite (𝒫 T) := Set.Finite.powerset T_finite
+  let f : FilterEqvQuotient M T → 𝒫 T :=
+    λ (X : FilterEqvQuotient M T) => Quotient.lift (λ x => ⟨{ φ ∈ T | x ⊧ φ }, (by simp_all)⟩) (by
+      intro x y hxy;
+      suffices {φ | φ ∈ T ∧ Satisfies M x φ} = {φ | φ ∈ T ∧ Satisfies M y φ} by simpa;
+      apply Set.eq_of_subset_of_subset;
+      . rintro φ ⟨hp, hx⟩; exact ⟨hp, (hxy φ hp).mp hx⟩;
+      . rintro φ ⟨hp, hy⟩; exact ⟨hp, (hxy φ hp).mpr hy⟩;
+      ) X
+  have hf : Function.Injective f := by
+    intro X Y h;
+    obtain ⟨x, rfl⟩ := Quotient.exists_rep X;
+    obtain ⟨y, rfl⟩ := Quotient.exists_rep Y;
+    simp [f] at h;
+    apply Quotient.eq''.mpr;
+    intro φ hp;
+    constructor;
+    . intro hpx;
+      have : ∀ a ∈ T, x ⊧ a → a ∈ T ∧ y ⊧ a := by simpa using h.subset;
+      exact this φ hp hpx |>.2;
+    . intro hpy;
+      have := h.symm.subset;
+      simp only [Set.setOf_subset_setOf, and_imp] at this;
+      exact this φ hp hpy |>.2;
+  exact Finite.of_injective f hf
+
+instance : Nonempty (FilterEqvQuotient M T) := ⟨⟦M.toFrame.world_nonempty.some⟧⟩
+
+end FilterEqvQuotient
+
+
+def toFilterEquivSet (X : Set M.World) : Set (FilterEqvQuotient M T) := { ⟦x⟧ | x ∈ X }
+local notation "【" X "】" => toFilterEquivSet X
+
+namespace toFilterEquivSet
+
+variable {X Y : Set M.World}
+
+@[grind]
+lemma mem_of_mem {x : M.World} (hx : x ∈ X) : ⟦x⟧ ∈ (【X】 : Set (FilterEqvQuotient M T)) := by use x;
+
+@[grind]
+lemma iff_mem_truthset (hφ : φ ∈ T) : x ∈ M.truthset φ ↔ ⟦x⟧ ∈ (【M.truthset φ】 : Set (FilterEqvQuotient M T)) := by
+  constructor;
+  . grind;
+  . rintro ⟨y, hy₁, hy₂⟩;
+    exact FilterEqvQuotient.iff_eq.mp hy₂ φ hφ |>.mp hy₁;
+
+
+@[simp, grind] lemma empty : (【∅】 : Set (FilterEqvQuotient M T)) = ∅ := by simp [toFilterEquivSet];
+
+@[grind]
+lemma union : (【X ∪ Y】 : Set (FilterEqvQuotient M T)) = (【X】 ∪ 【Y】 : Set (FilterEqvQuotient M T)) := by
+  ext Z;
+  constructor;
+  . rintro ⟨x, (hx | hx), rfl⟩;
+    . left; use x;
+    . right; use x;
+  . rintro (h | h) <;>
+    . obtain ⟨x, hx, rfl⟩ := h;
+      use x;
+      grind;
+
+lemma of_inter : (【X ∩ Y】 : Set (FilterEqvQuotient M T)) ⊆ (【X】 ∩ 【Y】 : Set (FilterEqvQuotient M T)) := by
+  rintro _ ⟨x, ⟨hx₁, hx₂⟩, rfl⟩;
+  constructor <;> use x;
+
+@[grind]
+lemma compl_truthset (hφ : φ ∈ T) : (【(M φ)ᶜ】 : Set (FilterEqvQuotient M T)) = 【M φ】ᶜ := by
+  ext X;
+  suffices (∃ x ∉ M.truthset φ, ⟦x⟧ = X) ↔ ∀ x ∈ M.truthset φ, ¬⟦x⟧ = X by simpa [toFilterEquivSet, Model.truthset];
+  constructor;
+  . rintro ⟨x, hx, rfl⟩ y hy;
+    apply FilterEqvQuotient.iff_eq.not.mpr;
+    push_neg;
+    use φ;
+    constructor;
+    . assumption;
+    . left; tauto;
+  . rintro h;
+    obtain ⟨x, rfl⟩ := Quotient.exists_rep X;
+    use x;
+    constructor;
+    . tauto;
+    . rfl;
+
+lemma subset_original_truthset_of_subset (hψ : ψ ∈ T) (h : (【M φ】 : Set (FilterEqvQuotient M T)) ⊆ 【M ψ】) : M φ ⊆ M ψ := by
+  intro x hx;
+  replace h : ∀ y ∈ M φ, ∃ z ∈ M ψ, (filterEquiv M T) z y := by simpa [toFilterEquivSet] using h;
+  obtain ⟨y, hy₁, hy₂⟩ := h x hx;
+  apply hy₂ ψ hψ |>.mp hy₁;
+
+lemma eq_original_truthset_of_eq (hφ : φ ∈ T) (hψ : ψ ∈ T) (h : (【M φ】 : Set (FilterEqvQuotient M T)) = 【M ψ】) : M φ = M ψ := by
+  apply Set.Subset.antisymm;
+  . apply toFilterEquivSet.subset_original_truthset_of_subset hψ; tauto_set;
+  . apply toFilterEquivSet.subset_original_truthset_of_subset hφ; tauto_set;
+
+
+lemma trans_truthset [M.IsTransitive] : (【M (□φ)】 : Set (FilterEqvQuotient M T)) ⊆ 【M (□□φ)】 := by
+  intro X;
+  suffices ∀ (x : M.World), x ∈ M (□φ) → ⟦x⟧ = X → ∃ x, M.box^[2] (M φ) x ∧ ⟦x⟧ = X by
+    simpa [toFilterEquivSet, Set.mem_setOf_eq];
+  rintro x hx rfl;
+  use x;
+  constructor;
+  . apply M.trans;
+    simpa;
+  . rfl;
+
+lemma refl_truthset [M.IsReflexive] : (【M (□φ)】 : Set (FilterEqvQuotient M T)) ⊆ 【M φ】 := by
+  intro X;
+  suffices ∀ (x : M.World), x ∈ M (□φ) → ⟦x⟧ = X → ∃ x, (M φ) x ∧ ⟦x⟧ = X by
+    simpa [toFilterEquivSet, Set.mem_setOf_eq];
+  rintro x hx rfl;
+  use x;
+  constructor;
+  . apply M.refl; simpa;
+  . rfl;
+
+lemma mono'_truthset [M.IsMonotonic] (hψ : ψ ∈ T) (h : (【M φ】 : Set (FilterEqvQuotient M T)) ⊆ 【M ψ】) : (【M (□φ)】 : Set (FilterEqvQuotient M T)) ⊆ 【M (□ψ)】 := by
+  intro X;
+  suffices ∀ (x : M.World), x ∈ M.truthset (□φ) → ⟦x⟧ = X → ∃ x, x ∈ M.truthset (□ψ) ∧ ⟦x⟧ = X by
+    simpa [toFilterEquivSet, Set.mem_setOf_eq];
+  rintro x hx rfl;
+  use x;
+  constructor;
+  . exact M.mono' (subset_original_truthset_of_subset hψ h) hx;
+  . rfl;
+
+end toFilterEquivSet
+
+
+structure Filtration (M : Model) (T : FormulaSet ℕ) [T.IsSubformulaClosed] where
+  B : Set (FilterEqvQuotient M T) → Set (FilterEqvQuotient M T)
+  B_def : ∀ φ, (□φ ∈ T) → B 【M φ】 = 【M.box (M φ)】
+  V : ℕ → Set (FilterEqvQuotient M T)
+  V_def : ∀ a, V a = 【M (.atom a)】
+
+namespace Filtration
+
+attribute [simp] Filtration.B_def Filtration.V_def
+
+variable {Fi : Filtration M T}
+
+def toModel {M : Model} {T : FormulaSet ℕ} [T.IsSubformulaClosed] (Fi : Filtration M T) : Model where
+  toFrame := Frame.mk_ℬ (FilterEqvQuotient M T) Fi.B
+  Val := Fi.V
+
+@[simp, grind]
+lemma toModel_def : Fi.toModel.box X = Fi.B X := by simp [Filtration.toModel, Frame.mk_ℬ, Frame.box]
+
+theorem filtration (Fi : Filtration M T) (φ) (hφ : φ ∈ T) : (Fi.toModel φ) = 【M φ】 := by
+  induction φ with
+  | hatom a => apply Fi.V_def;
+  | hfalsum => simp;
+  | himp φ ψ ihφ ihψ =>
+    replace ihφ := ihφ (by grind);
+    replace ihψ := ihψ (by grind);
+    simp_all [toFilterEquivSet.union, toFilterEquivSet.compl_truthset (show φ ∈ T by grind)];
+  | hbox φ ihφ =>
+    replace ihφ := ihφ (by grind);
+    apply ihφ ▸ Fi.B_def φ (by grind);
+
+lemma filtration_satisfies (Fi : Filtration M T) (φ) (hφ : φ ∈ T) {x : M} : Satisfies Fi.toModel ⟦x⟧ φ ↔ x ⊧ φ := by
+  simp only [Satisfies, (filtration Fi _ hφ)];
+  constructor;
+  . rintro ⟨y, hy, Ryx⟩;
+    simp only [FilterEqvSetoid, Quotient.eq, filterEquiv] at Ryx;
+    apply Ryx φ hφ |>.mp hy;
+  . tauto;
+
+lemma truthlemma (Fi : Filtration M T) {φ ψ} (hφ : φ ∈ T) (hψ : ψ ∈ T) :
+  (Fi.toModel φ) = (Fi.toModel ψ) ↔ (【M φ】 : Set (FilterEqvQuotient M T)) = (【M ψ】) := by
+  rw [filtration Fi φ hφ, filtration Fi ψ hψ];
+
+@[grind]
+lemma iff_mem_toModel_box_mem_B {Fi : Filtration M T} : W ∈ Fi.toModel.box Y ↔ W ∈ Fi.B Y := by
+  simp [Filtration.toModel, Frame.mk_ℬ, Frame.box];
+
+@[grind]
+lemma box_in_out {Fi : Filtration M T} (hφ : □φ ∈ T) : Fi.B 【M φ】 = 【M (□φ)】 := calc
+  _ = Fi.toModel.box 【M.truthset φ】 := by simp [Filtration.toModel, Frame.mk_ℬ, Frame.box];
+  _ = Fi.toModel.box (Fi.toModel φ) := by rw [filtration Fi φ (by grind)];
+  _ = (Fi.toModel (□φ)) := by simp;
+  _ = 【M (□φ)】 := filtration Fi _ hφ
+
+@[grind]
+lemma mem_box_in_out (hψ : □φ ∈ T) : X ∈ Fi.B 【M φ】 ↔ X ∈ 【M (□φ)】 := by grind;
+
+lemma transitive_lemma (hφ : φ ∈ T) (hψ : □ψ ∈ T) (Fi : Filtration M T) (h : 【M φ】 = Fi.B 【M ψ】) : (【M (□φ)】 : Set (FilterEqvQuotient M T)) = 【M (□□ψ)】 := by
+  have : M φ = M (□ψ) := toFilterEquivSet.eq_original_truthset_of_eq (T := T) hφ hψ $ (show 【M φ】 = 【M (□ψ)】 by exact Fi.box_in_out hψ ▸ h);
+  have : M.box (M φ) = M.box (M (□ψ)) := by rw [this];
+  have : M (□φ) = M (□□ψ) := by tauto;
+  tauto;
+
+end Filtration
+
+open Classical in
+def minimalFiltration (M : Model) (T : FormulaSet ℕ) [T.IsSubformulaClosed] : Filtration M T where
+  B X := if h : ∃ φ, □φ ∈ T ∧ X = 【M φ】 then 【M.box (M h.choose)】 else ∅
+  B_def := by
+    intro φ hφ;
+    split_ifs with hψ;
+    . suffices M φ = M hψ.choose by simp [←this];
+      have := hψ.choose_spec;
+      apply toFilterEquivSet.eq_original_truthset_of_eq (by grind) (by grind) this.2;
+    . push_neg at hψ;
+      have := hψ _ hφ;
+      contradiction;
+  V := λ a => 【M (.atom a)】
+  V_def := by intro a; rfl
+
+lemma minimalFiltration.iff_mem_B : W ∈ (minimalFiltration M T).B X ↔ ∃ φ, □φ ∈ T ∧ X = 【M.truthset φ】 ∧ W ∈ 【M.truthset (□φ)】 := by
+  constructor;
+  . intro h;
+    dsimp [minimalFiltration, Filtration.toModel, Frame.mk_ℬ, Frame.box] at h;
+    split_ifs at h with hY;
+    . use hY.choose;
+      refine ⟨?_, ?_, ?_⟩
+      . exact hY.choose_spec.1;
+      . exact hY.choose_spec.2;
+      . simpa;
+    . contradiction;
+  . rintro ⟨φ, hφ, rfl, hW⟩;
+    dsimp [minimalFiltration, Filtration.toModel, Frame.mk_ℬ, Frame.box];
+    split_ifs with h;
+    . suffices W ∈ 【M.truthset (□h.choose)】 by exact this;
+      exact (minimalFiltration M T).mem_box_in_out h.choose_spec.1 |>.mp $ h.choose_spec.2 ▸ (minimalFiltration M T).mem_box_in_out hφ |>.mpr hW;
+    . push_neg at h;
+      have := h φ hφ;
+      contradiction;
+
+
+open Classical in
+def transitiveFiltration (M : Model) [M.IsTransitive] (T : FormulaSet ℕ) [T.IsSubformulaClosed] : Filtration M T where
+  B X := ((minimalFiltration M T).B X) ∪ (if ∃ Y, X = (minimalFiltration M T).B Y then X else ∅)
+  B_def := by
+    intro φ hφ;
+    ext X;
+    constructor;
+    . rintro (hX | hX);
+      . exact (minimalFiltration M T).box_in_out hφ ▸ hX;
+      . split_ifs at hX with hY;
+        . obtain ⟨Y, hY⟩ : ∃ Y, 【M φ】 = if h : ∃ φ, □φ ∈ T ∧ Y = 【M φ】 then 【(M (□h.choose))】 else ∅ := hY;
+          split_ifs at hY with hZ;
+          . apply (minimalFiltration M T).transitive_lemma (φ := φ) (ψ := hZ.choose) ?_ ?_ ?_ ▸ (toFilterEquivSet.trans_truthset (hY ▸ hX));
+            . grind;
+            . exact hZ.choose_spec.1;
+            . exact minimalFiltration M T|>.box_in_out hZ.choose_spec.1 ▸ hY;
+          . tauto_set;
+        . contradiction;
+    . intro hX;
+      left;
+      suffices X ∈ if h : ∃ ψ, □ψ ∈ T ∧ 【M.truthset φ】 = 【M.truthset ψ】 then 【M.box (M h.choose)】 else ∅ by
+        simpa [Filtration.toModel, Frame.mk_ℬ, Model.truthset.eq_atom, Set.mem_setOf_eq];
+      split_ifs with h;
+      . have := h.choose_spec;
+        rwa [←(toFilterEquivSet.eq_original_truthset_of_eq (by grind) (by grind) this.2)];
+      . push_neg at h;
+        have := h _ hφ;
+        contradiction;
+  V := λ a => 【M (.atom a)】
+  V_def := by intro a; rfl
+
+
+namespace transitiveFiltration
+
+variable [M.IsTransitive]
+
+lemma iff_mem_B :
+  (W ∈ (transitiveFiltration M T).B X) ↔
+  (((∃ φ, □φ ∈ T ∧ X = 【M.truthset φ】 ∧ W ∈ 【M.truthset (□φ)】) ∨
+  (∃ φ, □φ ∈ T ∧ X = 【M.truthset (□φ)】 ∧ W ∈ 【M.truthset (□φ)】))) := by
+  constructor;
+  . rintro (h | h);
+    . left; exact minimalFiltration.iff_mem_B.mp h;
+    . split_ifs at h with hY;
+      . right;
+        obtain ⟨Y, rfl⟩ := hY;
+        obtain ⟨φ, hφ₁, rfl, hφ₃⟩ := minimalFiltration.iff_mem_B.mp h;
+        use φ;
+        refine ⟨hφ₁, ?_, ?_⟩;
+        . grind;
+        . assumption;
+      . contradiction;
+  . rintro (⟨φ, hφ₁, rfl, hφ₃⟩ | ⟨φ, hφ, rfl, _⟩);
+    . left;
+      apply minimalFiltration.iff_mem_B.mpr;
+      use φ;
+    . right;
+      suffices (∃ Y, 【M (□φ)】 = (minimalFiltration M T).B Y) ∧ W ∈ 【M (□φ)】 by simpa;
+      constructor;
+      . use (【M.truthset φ】);
+        rw [Filtration.box_in_out hφ]
+      . tauto;
+
+instance isTransitive : (transitiveFiltration M T).toModel.IsTransitive := by
+  constructor;
+  intro X;
+  by_cases h : (minimalFiltration M T).B X = ∅;
+  . simp_all [transitiveFiltration, Filtration.toModel, Frame.mk_ℬ, Frame.box];
+  . suffices (minimalFiltration M T).B X = (transitiveFiltration M T).B X by calc
+      _ = (transitiveFiltration M T).B X := by simp;
+      _ ⊆ (minimalFiltration M T).B X ∪ (minimalFiltration M T).B^[2] X := by tauto_set
+      _ ⊆ (transitiveFiltration M T).B ((minimalFiltration M T).B X) := by
+        rintro W (hW | hW);
+        . right;
+          split_ifs;
+          . assumption;
+          . grind;
+        . left; assumption;
+      _ = (transitiveFiltration M T).toModel.box^[2] X := by simp [this]
+    ext W;
+    constructor;
+    . tauto;
+    . rintro (hW | hW);
+      . assumption;
+      . split_ifs at hW with hif₁;
+        . obtain ⟨Y, hY⟩ := hif₁;
+          dsimp [minimalFiltration, Filtration.toModel, Frame.mk_ℬ, Frame.box] at hY;
+          split_ifs at hY with hif₂;
+          . generalize eψ : hif₂.choose = ψ at hif₂ hY;
+            have hψ : □ψ ∈ T := eψ ▸ hif₂.choose_spec.1;
+            replace hY : X = 【M (□ψ)】 := hY;
+            subst hY;
+            replace hW := toFilterEquivSet.trans_truthset hW;
+            obtain ⟨φ, hφ₁, hφ₂, _⟩ := by simpa [minimalFiltration, Filtration.toModel, Frame.mk_ℬ, Frame.box] using h;
+            have : (【M (□φ)】 : Set (FilterEqvQuotient M T)) = 【M (□□ψ)】 := (minimalFiltration M T).transitive_lemma (by grind) (by grind) $ by
+              rw [(minimalFiltration M T).box_in_out hψ];
+              exact hφ₂.symm;
+            rwa [←this, ←(Filtration.box_in_out (Fi := minimalFiltration M T) hφ₁), ←hφ₂] at hW;
+          . grind;
+        . grind;
+
+instance isReflexive [M.IsReflexive] : (transitiveFiltration M T).toModel.IsReflexive := by
+  constructor;
+  rintro X W hW;
+  rcases transitiveFiltration.iff_mem_B.mp hW with (⟨φ, hφ, rfl, _⟩ | ⟨φ, hφ, rfl, _⟩);
+  . apply toFilterEquivSet.refl_truthset;
+    assumption;
+  . assumption;
+
+end transitiveFiltration
+
+
+open Classical in
+def supplementedTransitiveFiltration (M : Model) [M.IsMonotonic] [M.IsTransitive] (T : FormulaSet ℕ) [T.IsSubformulaClosed] : Filtration M T where
+  B := (transitiveFiltration M T).toModel.supplementation.box
+  B_def := by
+    intro φ hφ;
+    suffices ⋃₀ {x | ∃ Y ⊆ 【M.truthset φ】, (transitiveFiltration M T).B Y = x} = 【M (□φ)】 by
+      simpa [Frame.supplementation.box_aux]
+    ext W;
+    constructor;
+    . rintro ⟨Y, ⟨Z, hZ₁, rfl⟩, hZ₂⟩;
+      rcases transitiveFiltration.iff_mem_B.mp hZ₂ with ⟨ψ, ψ_sub, rfl, hψ⟩ | ⟨ψ, ψ_sub, rfl, hψ⟩;
+      . exact toFilterEquivSet.mono'_truthset (by grind) (by assumption) hψ;
+      . apply toFilterEquivSet.mono'_truthset (by grind) (by assumption) $ toFilterEquivSet.trans_truthset hψ;
+    . intro hW;
+      use (transitiveFiltration M T).B 【M.truthset φ】;
+      constructor;
+      . use 【M.truthset φ】;
+      . exact (transitiveFiltration M T).mem_box_in_out hφ |>.mpr hW;
+  V := (transitiveFiltration M T).V
+  V_def := by simp;
+
+namespace supplementedTransitiveFiltration
+
+variable [M.IsMonotonic] [M.IsTransitive]
+
+protected instance isMonotonic: (supplementedTransitiveFiltration M T).toModel.IsMonotonic := ⟨
+  Frame.supplementation.isMonotonic (F := (transitiveFiltration M T).toModel.toFrame).mono
+⟩
+
+protected instance isTransitive : (supplementedTransitiveFiltration M T).toModel.IsTransitive := ⟨
+  Frame.supplementation.isTransitive (F := (transitiveFiltration M T).toModel.toFrame).trans
+⟩
+
+protected instance isReflexive [M.IsReflexive] : (supplementedTransitiveFiltration M T).toModel.IsReflexive := ⟨
+  Frame.supplementation.isReflexive (F := (transitiveFiltration M T).toModel.toFrame).refl
+⟩
+
+end supplementedTransitiveFiltration
+
+
+open Classical in
+def quasiFilteringTransitiveFiltration (M : Model) [M.IsMonotonic] [M.IsTransitive] [M.IsRegular] (T : FormulaSet ℕ) [T.IsSubformulaClosed] (hT : T.Finite) : Filtration M T where
+  V := (transitiveFiltration M T).V
+  V_def := by simp;
+  B := (transitiveFiltration M T).toModel.quasiFiltering.box
+  B_def := by
+    intro φ hφ;
+    ext W;
+    constructor;
+    . rintro ⟨Y, hY, ⟨Ys, hYs₁, hYs₂, hYs₃⟩⟩;
+      let Vs := { Vi ∈ Ys | ∃ ψ, □ψ ∈ T ∧ Vi = 【M ψ】 ∧ W ∈ 【M (□ψ)】 };
+      let Us := { Ui ∈ Ys | ∃ ψ, □ψ ∈ T ∧ Ui = 【M (□ψ)】 ∧ W ∈ 【M (□ψ)】 };
+      have eYVU : Ys = Vs ∪ Us := by
+        ext Yi;
+        simp only [Finset.mem_union, Finset.mem_filter, Vs, Us];
+        constructor;
+        . intro hYi;
+          rcases transitiveFiltration.iff_mem_B.mp $ hYs₃ Yi hYi with (hV | hU);
+          . left; tauto;
+          . right; tauto;
+        . tauto_set;
+
+      let Ψ := {ψ // □ψ ∈ T ∧ (∃ Vi ∈ Ys, Vi = 【M ψ】) ∧ W ∈ 【M (□ψ)】};
+      have : Fintype Ψ := by
+        apply Fintype.subtype (s := { ψ ∈ hT.toFinset.prebox | (∃ Vi ∈ Ys, Vi = 【M ψ】) ∧ W ∈ 【M (□ψ)】 });
+        simp;
+      let Ξ := {ξ // □ξ ∈ T ∧ (∃ Ui ∈ Ys, Ui = 【M (□ξ)】) ∧ W ∈ 【M (□ξ)】};
+      have : Fintype Ξ := by
+        apply Fintype.subtype (s := { ξ ∈ hT.toFinset.prebox | (∃ Ui ∈ Ys, Ui = 【M (□ξ)】) ∧ W ∈ 【M (□ξ)】 });
+        simp;
+
+      have H : (⋂ ψ : Ψ, 【M ψ】) ∩ (⋂ ξ : Ξ, 【M (□ξ)】) ⊆ (【M φ】 : Set (FilterEqvQuotient M T)) := by calc
+        _ = (⋂ ψ : Ψ, 【M ψ】) ∩ (⋂ Ui ∈ Us, Ui) := by
+          suffices (⋂ ψ : Ξ, 【M (□ψ)】) = (⋂ Ui ∈ Us, Ui) by congr;
+          ext A;
+          suffices
+            (∀ ξ, □ξ ∈ T → 【M (□ξ)】 ∈ Ys → W ∈ 【M (□ξ)】 → A ∈ 【M (□ξ)】) ↔
+            (∀ ξ, □ξ ∈ T → ∀ Yi ∈ Ys, Yi = 【M (□ξ)】 → W ∈ 【M (□ξ)】 → A ∈ Yi) by
+            simp [Ξ, Us];
+            tauto;
+          constructor;
+          . rintro h _ _ _ _ rfl;
+            apply h <;> assumption;
+          . rintro h _ _ _ _;
+            apply h <;> tauto;
+        _ = (⋂ Vi ∈ Vs, Vi) ∩ (⋂ Ui ∈ Us, Ui) := by
+          suffices (⋂ ψ : Ψ, 【M ψ】) = (⋂ Vi ∈ Vs, Vi) by congr;
+          ext A;
+          suffices
+            (∀ ψ, □ψ ∈ T → 【M ψ】 ∈ Ys → W ∈ 【M (□ψ)】 → A ∈ 【M ψ】) ↔
+            (∀ ψ, □ψ ∈ T → ∀ Yi ∈ Ys, Yi = 【M ψ】 → W ∈ 【M (□ψ)】 → A ∈ Yi) by
+            simp [Ψ, Vs];
+            tauto;
+          constructor;
+          . rintro h _ _ _ _ rfl;
+            apply h <;> assumption;
+          . rintro h _ _ _ _;
+            apply h <;> tauto;
+        _ = ⋂ Xi ∈ Ys, Xi := by
+          ext A;
+          simp only [Set.mem_inter_iff, Set.mem_iInter, eYVU, Finset.mem_union];
+          constructor;
+          . rintro ⟨hV, hU⟩ i (hi | hi);
+            . exact hV i hi;
+            . exact hU i hi;
+          . rintro h;
+            constructor;
+            . intro i hi;
+              apply h;
+              left;
+              assumption;
+            . intro i hi;
+              apply h;
+              right;
+              assumption;
+        _ = Y             := by grind;
+        _ ⊆ 【M φ】         := by assumption;
+      obtain ⟨w, rfl⟩ := Quotient.exists_rep W;
+      by_cases hΨ : Nonempty Ψ <;> by_cases hΞ : Nonempty Ξ;
+      . suffices w ∈ M.box ((⋂ ψ : Ψ, M ψ) ∩ (⋂ ξ : Ξ, M (□ξ))) by
+          apply toFilterEquivSet.mem_of_mem;
+          replace H : M.box ((⋂ ψ : Ψ, M ψ) ∩ (⋂ ξ : Ξ, M (□ξ))) ⊆ M.box (M φ) := M.mono' $ by
+            rintro a ⟨haψ, haξ⟩;
+            apply toFilterEquivSet.iff_mem_truthset (T := T) (by grind) |>.mpr;
+            apply H;
+            constructor;
+            . apply Set.mem_iInter.mpr;
+              intro ψ;
+              apply toFilterEquivSet.iff_mem_truthset (by grind) |>.mp;
+              apply haψ;
+              simp;
+            . apply Set.mem_iInter.mpr;
+              intro ξ;
+              apply toFilterEquivSet.iff_mem_truthset (by grind) |>.mp;
+              apply haξ;
+              simp;
+          apply H this;
+        apply M.regular;
+        constructor;
+        . suffices ∀ ψ : Ψ, w ∈ M (□ψ) by apply M.regular_finite_iUnion; simpa;
+          rintro ⟨ψ, _, ⟨Vi, hVi, rfl⟩, ⟨v, hv₁, hv₂⟩⟩;
+          grind;
+        . suffices ∀ ξ : Ξ, w ∈ M (□^[2]ξ) by apply M.regular_finite_iUnion (ι := Ξ); simpa;
+          rintro ⟨ξ, _, ⟨Ui, hUi, rfl⟩, ⟨v, hv₁, hv₂⟩⟩;
+          replace hv₁ : v ∈ M.box^[2] (M ξ) := M.trans hv₁;
+          grind;
+      . suffices ∀ ψ : Ψ, w ∈ M (□ψ) by
+          apply toFilterEquivSet.mem_of_mem;
+          replace H : M.box (⋂ ψ : Ψ, M ψ) ⊆ M.box (M φ) := M.mono' $ by
+            rintro a haψ;
+            apply toFilterEquivSet.iff_mem_truthset (T := T) (by grind) |>.mpr;
+            apply H;
+            constructor;
+            . apply Set.mem_iInter.mpr;
+              intro ψ;
+              apply toFilterEquivSet.iff_mem_truthset (by grind) |>.mp;
+              apply haψ;
+              simp;
+            . have : ⋂ ξ : Ξ, (【M.truthset (□ξ)】 : Set (FilterEqvQuotient M T)) = Set.univ := by
+                ext A;
+                simp [@IsEmpty.forall_iff (α := Ξ) (by simpa using hΞ)];
+              rw [this];
+              simp;
+          apply H;
+          apply M.regular_finite_iUnion;
+          simpa;
+        rintro ⟨ψ, _, ⟨Vi, hVi, rfl⟩, ⟨v, hv₁, hv₂⟩⟩;
+        grind;
+      . suffices ∀ ξ : Ξ, w ∈ M (□^[2]ξ) by
+          apply toFilterEquivSet.mem_of_mem;
+          replace H : M.box (⋂ ξ : Ξ, M (□ξ)) ⊆ M.box (M φ) := M.mono' $ by
+            rintro a haξ;
+            apply toFilterEquivSet.iff_mem_truthset (T := T) (by grind) |>.mpr;
+            apply H;
+            constructor;
+            . have : ⋂ ψ : Ψ, (【M.truthset ψ】 : Set (FilterEqvQuotient M T)) = Set.univ := by
+                ext A;
+                simp [@IsEmpty.forall_iff (α := Ψ) (by simpa using hΨ)];
+              rw [this];
+              simp;
+            . apply Set.mem_iInter.mpr;
+              intro ξ;
+              apply toFilterEquivSet.iff_mem_truthset (by grind) |>.mp;
+              apply haξ;
+              simp;
+          apply H;
+          apply M.regular_finite_iUnion;
+          simpa;
+        rintro ⟨ξ, _, ⟨Ui, hUi, rfl⟩, ⟨v, hv₁, hv₂⟩⟩;
+        replace hv₁ : v ∈ M.box^[2] (M ξ) := M.trans hv₁;
+        grind;
+      . exfalso;
+        apply hYs₁;
+        suffices (Vs = ∅ ∧ Us = ∅) by simp [eYVU, this.1, this.2];
+        constructor;
+        . suffices ∀ Yi ∈ Ys, ∀ ψ, □ψ ∈ T → Yi = 【M ψ】 → ⟦w⟧ ∉ 【M (□ψ)】 by simpa [Vs];
+          rintro _ _ ψ hψ rfl;
+          apply (show ∀ ψ, □ψ ∈ T → 【M ψ】 ∈ Ys → ⟦w⟧ ∉ 【M (□ψ)】 by simpa [Ψ] using hΨ) <;> assumption;
+        . suffices ∀ Yi ∈ Ys, ∀ ξ, □ξ ∈ T → Yi = 【M (□ξ)】 → ⟦w⟧ ∉ 【M (□ξ)】 by simpa [Us];
+          rintro _ _ ξ hξ rfl;
+          apply (show ∀ ξ, □ξ ∈ T → 【M (□ξ)】 ∈ Ys → ⟦w⟧ ∉ 【M (□ξ)】 by simpa [Ξ] using hΞ) <;> assumption;
+    . intro h;
+      apply Frame.quasiFiltering.mem_box_of_mem_original_box;
+      apply transitiveFiltration.iff_mem_B.mpr;
+      left;
+      use φ;
+      tauto;
+
+namespace quasiFilteringTransitiveFiltration
+
+variable {T_finite : Set.Finite T} [M.IsMonotonic] [M.IsTransitive] [M.IsRegular]
+
+protected instance isRegular : (quasiFilteringTransitiveFiltration M T T_finite).toModel.IsRegular := ⟨
+  Frame.quasiFiltering.isRegular (F := (transitiveFiltration M T).toModel.toFrame).regular
+⟩
+
+protected instance isMonotonic: (quasiFilteringTransitiveFiltration M T T_finite).toModel.IsMonotonic := ⟨
+  Frame.quasiFiltering.isMonotonic (F := (transitiveFiltration M T).toModel.toFrame).mono
+⟩
+
+protected instance isTransitive : (quasiFilteringTransitiveFiltration M T T_finite).toModel.IsTransitive := ⟨
+  Frame.quasiFiltering.isTransitive (F := (transitiveFiltration M T).toModel.toFrame).trans
+⟩
+
+end quasiFilteringTransitiveFiltration
+
+end Neighborhood
+
+end LO.Modal
